@prefix rdf: <http://www.w3.org/1999/02/22-rdf-syntax-ns#> .
@prefix rdfs: <http://www.w3.org/2000/01/rdf-schema#> .
@prefix xsd:  <http://www.w3.org/2001/XMLSchema#>.
@prefix owl: <http://www.w3.org/2002/07/owl#> .
@prefix foaf: <http://xmlns.com/foaf/0.1/> .
@prefix dbp: <http://dbpedia.org/resource/> .
@prefix ontology: <https://raw.githubusercontent.com/JiriResler/dietary-profile-and-customized-menus-resources/main/ontology#> .

#### Ontology ####
ontology:
  a owl:Ontology ;
  rdfs:label "Dietary profile and customized menus ontology"@en ;
  rdfs:comment "Ontology describes the classes and properties used by the suite of applications to display customized restaurant menus to guests based on their dietary profiles."@en .

#### Classes ####
ontology:DietaryProfile
  a foaf:PersonalProfileDocument ;
  rdfs:label "Dietary profile"@en ;
  rdfs:comment "Dietary profile of a foaf:Person containing their allergies, diets, and taste preferences."@en .

ontology:Diet 
  a rdfs:Class ;
  rdfs:label "Diet"@en ;
  rdfs:comment "Diet as when someone eats only specific types of food due to health reasons or personal beliefs."@en ;
  owl:sameAs <http://dbpedia.org/resource/Diet_(nutrition)> .

ontology:NationalCuisine
  a rdfs:Class ;
  rdfs:label "National cuisine"@en ;
  rdfs:comment "Cuisine specific to a particular country."@en ;
  owl:sameAs <http://www.wikidata.org/entity/Q1968435> .

#### Properties ####
ontology:allergicTo
  a rdf:Property ;
  rdfs:label "Allergic to"@en ;
  rdfs:comment "Specifies that a foaf:Person is allergic to a ontology:Allergen."@en ;
  rdfs:domain foaf:Person ;
  rdfs:range ontology:Allergen .

ontology:onDiet
  a rdf:Property ;
  rdfs:label "On diet"@en ;
  rdfs:comment "Specifies that a foaf:Person is on a ontology:Diet."@en ;
  rdfs:domain foaf:Person ;
  rdfs:range ontology:Diet .

ontology:likesTasteOf
  a rdf:Property ;
  rdfs:label "Likes taste of"@en ;
  rdfs:comment "Specifies that a foaf:Person likes the taste of something."@en ;
  rdfs:domain foaf:Person .

ontology:prefersDessertTaste
  a rdf:Property ;
  rdfs:label "Prefers dessert taste"@en ;
  rdfs:comment "Specifies that a foaf:Person prefers a specific taste of desserts."@en ;
  rdfs:domain foaf:Person ;
  rdfs:range 
    [
      a rdf:Alt ;
      rdf:_1 "sweet" ;
      rdf:_2 "savory" ;
    ] .

ontology:preferesLevelOfSpiciness
  a rdf:Property ;
  rdfs:label "Prefers level of spiciness"@en ;
  rdfs:comment "Specifies how spicy a foaf:Person prefers their food to be."@en ;
  rdfs:domain foaf:Person ;
  rdfs:range 
    [
      a rdf:Alt ;
      rdf:_1 "mild" ;
      rdf:_2 "medium" ;
      rdf:_3 "medium-hot" ;
      rdf:_4 "hot" ;
      rdf:_5 "extra hot" ;
    ] .

ontology:howOftenAddsSalt
  a rdf:Property ;
  rdfs:label "How often adds salt"@en ;
  rdfs:comment "Specifies how often a foaf:Person adds additional salt to their food if it is prepared by someone else."@en ;
  rdfs:domain foaf:Person ;
  rdfs:range 
    [
      a rdf:Alt ;
      rdf:_1 "never" ;
      rdf:_2 "sometimes" ;
      rdf:_3 "often" ;
      rdf:_4 "always" ;
    ] .

ontology:allergenNumber
  a rdf:Property ;
  rdfs:label "Allergen number"@en ;
  rdfs:comment "A number which is used identify a specific allergen."@en ;
  rdfs:domain dbp:Allergen ;
  rdfs:range xsd:integer .

ontology:allergenIcon
  a rdf:Property ;
  rdfs:label "Has allergen icon"@en ;
  rdfs:comment "The URL of a file which contains an image of the allergen."@en ;
  rdfs:domain ontology:Allergen ;
  rdfs:range foaf:Image .
