@prefix rdf: <http://www.w3.org/1999/02/22-rdf-syntax-ns#> .
@prefix rdfs: <http://www.w3.org/2000/01/rdf-schema#> .
@prefix xsd:  <http://www.w3.org/2001/XMLSchema#>.
@prefix owl: <http://www.w3.org/2002/07/owl#> .
@prefix foaf: <http://xmlns.com/foaf/0.1/> .
@prefix ontology: <https://raw.githubusercontent.com/JiriResler/dietary-profile-and-customized-menus-resources/main/ontology#> .

#### Ontology ####
ontology:
  a owl:Ontology ;
  rdfs:label "Dietary profile and customized menus ontology"@en ;
  rdfs:comment "Ontology describes the classes and properties used by the suite of applications to display customized restaurant menus to guests based on their dietary profiles."@en .

#### Classes ####
ontology:DietaryProfile
  a foaf:PersonalProfileDocument ;
  rdfs:label "Dietary profile"@en ;
  rdfs:comment "Dietary profile of a foaf:Person containing their allergies, diets, and taste preferences."@en .

ontology:Allergen 
  a rdfs:Class ;
  rdfs:label "Allergen"@en ;
  rdfs:comment "Allergen which can be found in food ingredients."@en ;
  owl:sameAs <http://dbpedia.org/resource/Allergen> .

ontology:Diet 
  a rdfs:Class ;
  rdfs:label "Diet"@en ;
  rdfs:comment "Diet as when someone eats only specific types of food due to health reasons or personal beliefs."@en ;
  owl:sameAs <http://dbpedia.org/resource/Diet_(nutrition)> .

ontology:Cuisine
  a rdfs:Class ;
  rdfs:label "Cuisine"@en ;
  rdfs:comment "Cuisine specific to a particular region of the world."@en ;
  owl:sameAs <http://dbpedia.org/resource/Category:Cuisine> .

ontology:Sauce
  a rdfs:Class ;
  rdfs:label "Sauce"@en ;
  rdfs:comment "Sauce used as a separate addition to a dish."@en ;
  owl:sameAs <http://dbpedia.org/resource/Sauce> .

#### Properties ####
ontology:allergicTo
  a rdf:Property ;
  rdfs:label "Allergic to"@en ;
  rdfs:comment "Specifies that a foaf:Person is allergic to a ontology:Allergen."@en ;
  rdfs:domain foaf:Person ;
  rdfs:range ontology:Allergen .

ontology:onDiet
  a rdf:Property ;
  rdfs:label "On diet"@en ;
  rdfs:comment "Specifies that a foaf:Person is on a ontology:Diet."@en ;
  rdfs:domain foaf:Person ;
  rdfs:range ontology:Diet .

ontology:likesCuisine
  a rdf:Property ;
  rdfs:label "Likes cuisine"@en ;
  rdfs:comment "Specifies that a foaf:Person likes a ontology:Cuisine."@en ;
  rdfs:domain foaf:Person ;
  rdfs:range ontology:Cuisine .

ontology:prefersDessertTaste
  a rdf:Property ;
  rdfs:label "Prefers dessert taste"@en ;
  rdfs:comment "Specifies that a foaf:Person prefers a specific taste of desserts."@en ;
  rdfs:domain foaf:Person ;
  rdfs:range 
    [
      a rdf:Alt ;
      rdf:_1 "sweet" ;
      rdf:_2 "savory" ;
    ] .

ontology:preferesLevelOfSpiciness
  a rdf:Property ;
  rdfs:label "Prefers level of spiciness"@en ;
  rdfs:comment "Specifies how spicy a foaf:Person prefers their food to be, if they eat spicy food at all."@en ;
  rdfs:domain foaf:Person ;
  rdfs:range 
    [
      a rdf:Alt ;
      rdf:_1 "mild" ;
      rdf:_2 "medium" ;
      rdf:_3 "medium-hot" ;
      rdf:_4 "hot" ;
      rdf:_5 "extra hot" ;
    ] .

ontology:allergenNumber
  a rdf:Property ;
  rdfs:label "Allergen number"@en ;
  rdfs:comment "A number which is used in restaurant menus to identify a specific allergen."@en ;
  rdfs:domain ontology:Allergen ;
  rdfs:range xsd:integer .

ontology:hasIcon
  a rdf:Property ;
  rdfs:label "Has icon"@en ;
  rdfs:comment "The URL of a file which contains an image of the allergen."@en ;
  rdfs:domain ontology:Allergen ;
  rdfs:range foaf:Image .
