@prefix rdf: <http://www.w3.org/1999/02/22-rdf-syntax-ns#> .
@prefix rdfs: <http://www.w3.org/2000/01/rdf-schema#> .
@prefix xsd:  <http://www.w3.org/2001/XMLSchema#>.
@prefix owl: <http://www.w3.org/2002/07/owl#> .
@prefix dcterms: <http://purl.org/dc/terms/> .
@prefix vann: <http://purl.org/vocab/vann/> .
@prefix foaf: <http://xmlns.com/foaf/0.1/> .
@prefix ontology: <https://raw.githubusercontent.com/JiriResler/personalized-restaurant-menu-viewer-application-ontology/main/ontology#> .
@prefix schema: <https://schema.org/> .

ontology:
  a owl:Ontology ;
  dcterms:title "Personal restaurant menu viewer application ontology"@en ;
  dcterms:description "The ontology describing classes and properties used by applications which work with personal eating preferences of users."@en ;
  vann:preferredNamespacePrefix "eatingPreferences" .

ontology:Allergen 
  a rdfs:Class ;
  rdfs:label "Allergen"@en ;
  rdfs:comment "An allergen"@en ;
  owl:sameAs <http://dbpedia.org/resource/Allergen> .

ontology:allergenNumber
  a rdf:Property ;
  rdfs:label "Allergen number"@en ;
  dcterms:description "A number which is used in restaurant menus to identify a specific allergen"@en ;
  rdfs:domain ontology:Allergen ;
  rdfs:range xsd:integer .

ontology:hasIcon
  a rdf:Property ;
  rdfs:label "Has icon"@en ;
  dcterms:description "The URL of a file which contains an image of the allergen"@en ;
  rdfs:domain ontology:Allergen ;
  rdfs:range foaf:Image .

ontology:List_of_most_common_allergens
  a rdf:Seq ;
  rdfs:label "List of most common allergens"@en ;
  dcterms:description "A list of most common allergens defined by the European Union. There are currently 14 allergens in the list."@en ;
  schema:url <https://raw.githubusercontent.com/JiriResler/personalized-restaurant-menu-viewer-application-ontology/main/resource/List_of_most_common_allergens> .

ontology:allergicTo
  a rdf:Property ;
  rdfs:label "Allergic to"@en ;
  rdfs:domain foaf:Person ;
  rdfs:range ontology:Allergen .
